Extracted certT into separate file

src/cert_graph/Cert_tc.v
@@ -25,6 +25,7 @@ From imm Require Import TLSCoherency.
 From imm Require Import IordCoherency.
 Require Import TlsEventSets.
 Require Import EventsTraversalOrder.
+Require Import CertT.
 
 Require Import ExtTraversalConfig.
 
@@ -278,98 +279,6 @@ Notation "'CAcq/Rel'" := (fun a => is_true (is_ra Clab a)).
 Notation "'CSc'" := (fun a => is_true (is_sc Clab a)).
 
 
-Definition certT :=
-  (T ∪₁ eq ta_cover <*> (E ∩₁ NTid_ thread)) \₁ action ↓₁ eq ta_reserve ∪₁
-  eq ta_reserve <*> (issued T ∪₁ reserved T ∩₁ Tid_ thread). 
-
-Lemma tls_cover_certT:
-  certT ∩₁ action ↓₁ eq ta_cover ≡₁
-  (T ∪₁ event ↓₁ (E ∩₁ NTid_ thread)) ∩₁ action ↓₁ eq ta_cover. 
-Proof using. 
-  unfold certT. rewrite !set_pair_alt. fold action event.
-  rewrite set_minus_union_l, !set_inter_union_l.
-  rewrite set_equiv_union with (t' := ∅); [| reflexivity| ].  
-  2: { split; [| basic_solver]. iord_dom_solver. }
-  rewrite set_union_empty_r. apply set_equiv_union.
-  all: split; [basic_solver| iord_dom_solver]. 
-Qed. 
-
-Lemma covered_certT:
-  covered certT ≡₁ C ∪₁ E ∩₁ NTid_ thread. 
-Proof using.
-  (* it's just easier to prove it separately without appealing to tls_cover_certT *)
-  clear. 
-  unfold certT. simplify_tls_events. basic_solver 10.
-Qed. 
-  
-Lemma tls_issue_certT:
-  certT ∩₁ action ↓₁ eq ta_issue ≡₁ T ∩₁ action ↓₁ eq ta_issue. 
-Proof using. 
-  unfold certT. rewrite !set_pair_alt. fold action event.
-  rewrite set_minus_union_l, !set_inter_union_l.
-  rewrite set_equiv_union with (t' := ∅); [rewrite set_union_empty_r| reflexivity| ].
-  2: { split; [| basic_solver]. iord_dom_solver. }
-  rewrite set_equiv_union with (t' := ∅); [rewrite set_union_empty_r| reflexivity| ]. 
-  2: { split; [| basic_solver]. iord_dom_solver. }
-  split; [basic_solver| iord_dom_solver]. 
-Qed. 
-
-Lemma issued_certT:
-  issued certT ≡₁ I. 
-Proof using.
-  clear. 
-  unfold certT. simplify_tls_events. basic_solver 10. 
-Qed. 
-  
-Lemma reserved_certT:
-  reserved certT ≡₁ issued T ∪₁ reserved T ∩₁ Tid_ thread. 
-Proof using.
-  clear. 
-  unfold certT. simplify_tls_events.
-  rewrite set_minus_absorb_l; [basic_solver| ]. 
-  unfold reserved. unfolder. ins. desc. vauto.   
-Qed. 
-
-Lemma T_propagations_certT_thread t:
-  certT ∩₁ action ↓₁ (eq (ta_propagate t)) ≡₁
-  T ∩₁ action ↓₁ (eq (ta_propagate t)).
-Proof using.
-  clear. 
-  unfold certT. simplify_tls_events.
-  rewrite !set_pair_alt. fold action event. 
-  rewrite set_minus_union_l, !set_inter_union_l.
-  rewrite set_unionA, set_equiv_union with (t' := ∅). 
-  2: { rewrite set_minusE, set_interA.
-       rewrite set_interC with (s := set_compl _).
-       rewrite set_inter_absorb_r with (s := action ↓₁ _); [reflexivity| ].
-       unfolder. by intros ? <-. }
-  2: { split; [| basic_solver].
-       unfolder. ins; des; vauto; congruence. }
-  basic_solver.
-Qed.  
-
-
-Lemma T_propagations_certT:
-  certT ∩₁ action ↓₁ (is_ta_propagate_to_G G) ≡₁
-  T ∩₁ action ↓₁ (is_ta_propagate_to_G G).
-Proof using.
-  unfold is_ta_propagate_to_G.
-  rewrite set_map_bunion, <- !set_bunion_inter_compat_l.
-  apply set_equiv_bunion; [done| ].
-  ins. apply T_propagations_certT_thread. 
-Qed. 
-
-Lemma propagated_thread_certT t:
-  propagated_thread certT t ≡₁ propagated_thread T t.
-Proof using. 
-  unfold propagated_thread. by rewrite T_propagations_certT_thread. 
-Qed. 
-
-Lemma propagated_certT: propagated G certT ≡₁ propagated G T.
-Proof using.
-  unfold propagated. by rewrite T_propagations_certT. 
-Qed. 
-
 Lemma certG_same_props:
   is_ta_propagate_to_G certG ≡₁ is_ta_propagate_to_G G. 
 Proof using. auto. Qed. 
@@ -393,21 +302,6 @@ Lemma exec_tls_cert:
 Proof using SAME. 
   unfold exec_tls. rewrite cert_E. erewrite cert_W; eauto. 
 Qed.  
-
-Lemma certT_alt:
-  certT ≡₁ T ∩₁ action ↓₁ (eq ta_cover ∪₁ eq ta_issue ∪₁
-                     is_ta_propagate) ∪₁
-    (eq ta_reserve <*> (I ∪₁ S ∩₁ Tid_ thread)) ∪₁
-    ((eq ta_cover) <*> (E ∩₁ NTid_ thread)). 
-Proof using.
-  clear. 
-  unfold certT. rewrite !set_pair_alt. apply AuxRel.set_equiv_exp_equiv.
-  unfolder. intros [t a]. split; ins; des; destruct t; ins; splits. 
-  all: try (by vauto || tauto).
-  all: try by (repeat left; vauto). 
-  { left. right. vauto. }
-  right. vauto.
-Qed.  
   
 Lemma cert_imm_consistent (FAIR: mem_fair G):
   imm_consistent certG sc.
@@ -427,6 +321,7 @@ Proof using E_F_AcqRel_in_C E_to_S F_in_C RELCOV S_in_W WF TCOH ICOH.
   generalize E_F_AcqRel_in_C; basic_solver 12.
 Qed.  
   
+Notation "'certT'" := (certT G T thread). 
  
 
 Lemma TCOH_cert:
