src/cert_graph/CertT.v
@@ -1,0 +1,135 @@
+From hahn Require Import Hahn.
+From imm Require Import Events.
+From imm Require Import Execution.
+From imm Require Import TraversalOrder.
+From imm Require Import TLSCoherency.
+From imm Require Import IordCoherency.
+Require Import TlsEventSets.
+Require Import EventsTraversalOrder.
+From imm Require Import AuxDef.
+Require Import CertExecution2.
+
+Section CertT.
+Variables (G: execution) (sc: relation actid) (T: trav_label -> Prop). 
+Variable (thread: BinNums.positive). 
+
+Notation "'Init'" := (fun a => is_true (is_init a)).
+Notation "'E'" := (acts_set G).
+Notation "'NTid_' t" := (fun x => tid x <> t) (at level 1).
+Notation "'Tid_' t" := (fun x => tid x = t) (at level 1).
+
+Notation "'I'" := (issued T).
+Notation "'C'" := (covered T).
+Notation "'S'" := (reserved T).
+
+
+
+Definition certT :=
+  (T ∪₁ eq ta_cover <*> (E ∩₁ NTid_ thread)) \₁ action ↓₁ eq ta_reserve ∪₁
+  eq ta_reserve <*> (issued T ∪₁ reserved T ∩₁ Tid_ thread). 
+
+Lemma tls_cover_certT:
+  certT ∩₁ action ↓₁ eq ta_cover ≡₁
+  (T ∪₁ event ↓₁ (E ∩₁ NTid_ thread)) ∩₁ action ↓₁ eq ta_cover. 
+Proof using. 
+  unfold certT. rewrite !set_pair_alt. fold action event.
+  rewrite set_minus_union_l, !set_inter_union_l.
+  rewrite set_equiv_union with (t' := ∅); [| reflexivity| ].  
+  2: { split; [| basic_solver]. iord_dom_solver. }
+  rewrite set_union_empty_r. apply set_equiv_union.
+  all: split; [basic_solver| iord_dom_solver]. 
+Qed. 
+
+Lemma covered_certT:
+  covered certT ≡₁ C ∪₁ E ∩₁ NTid_ thread. 
+Proof using.
+  (* it's just easier to prove it separately without appealing to tls_cover_certT *)
+  clear. 
+  unfold certT. simplify_tls_events. basic_solver 10.
+Qed. 
+  
+Lemma tls_issue_certT:
+  certT ∩₁ action ↓₁ eq ta_issue ≡₁ T ∩₁ action ↓₁ eq ta_issue. 
+Proof using. 
+  unfold certT. rewrite !set_pair_alt. fold action event.
+  rewrite set_minus_union_l, !set_inter_union_l.
+  rewrite set_equiv_union with (t' := ∅); [rewrite set_union_empty_r| reflexivity| ].
+  2: { split; [| basic_solver]. iord_dom_solver. }
+  rewrite set_equiv_union with (t' := ∅); [rewrite set_union_empty_r| reflexivity| ]. 
+  2: { split; [| basic_solver]. iord_dom_solver. }
+  split; [basic_solver| iord_dom_solver]. 
+Qed. 
+
+Lemma issued_certT:
+  issued certT ≡₁ I. 
+Proof using.
+  clear. 
+  unfold certT. simplify_tls_events. basic_solver 10. 
+Qed. 
+  
+Lemma reserved_certT:
+  reserved certT ≡₁ issued T ∪₁ reserved T ∩₁ Tid_ thread. 
+Proof using.
+  clear. 
+  unfold certT. simplify_tls_events.
+  rewrite set_minus_absorb_l; [basic_solver| ]. 
+  unfold reserved. unfolder. ins. desc. vauto.   
+Qed. 
+
+Lemma T_propagations_certT_thread t:
+  certT ∩₁ action ↓₁ (eq (ta_propagate t)) ≡₁
+  T ∩₁ action ↓₁ (eq (ta_propagate t)).
+Proof using.
+  clear. 
+  unfold certT. simplify_tls_events.
+  rewrite !set_pair_alt. fold action event. 
+  rewrite set_minus_union_l, !set_inter_union_l.
+  rewrite set_unionA, set_equiv_union with (t' := ∅). 
+  2: { rewrite set_minusE, set_interA.
+       rewrite set_interC with (s := set_compl _).
+       rewrite set_inter_absorb_r with (s := action ↓₁ _); [reflexivity| ].
+       unfolder. by intros ? <-. }
+  2: { split; [| basic_solver].
+       unfolder. ins; des; vauto; congruence. }
+  basic_solver.
+Qed.  
+
+
+Lemma T_propagations_certT:
+  certT ∩₁ action ↓₁ (is_ta_propagate_to_G G) ≡₁
+  T ∩₁ action ↓₁ (is_ta_propagate_to_G G).
+Proof using.
+  unfold is_ta_propagate_to_G.
+  rewrite set_map_bunion, <- !set_bunion_inter_compat_l.
+  apply set_equiv_bunion; [done| ].
+  ins. apply T_propagations_certT_thread. 
+Qed. 
+
+Lemma propagated_thread_certT t:
+  propagated_thread certT t ≡₁ propagated_thread T t.
+Proof using. 
+  unfold propagated_thread. by rewrite T_propagations_certT_thread. 
+Qed. 
+
+Lemma propagated_certT: propagated G certT ≡₁ propagated G T.
+Proof using.
+  unfold propagated. by rewrite T_propagations_certT. 
+Qed. 
+
+
+Lemma certT_alt:
+  certT ≡₁ T ∩₁ action ↓₁ (eq ta_cover ∪₁ eq ta_issue ∪₁
+                     is_ta_propagate) ∪₁
+    (eq ta_reserve <*> (I ∪₁ S ∩₁ Tid_ thread)) ∪₁
+    ((eq ta_cover) <*> (E ∩₁ NTid_ thread)). 
+Proof using.
+  clear. 
+  unfold certT. rewrite !set_pair_alt. apply AuxRel.set_equiv_exp_equiv.
+  unfolder. intros [t a]. split; ins; des; destruct t; ins; splits. 
+  all: try (by vauto || tauto).
+  all: try by (repeat left; vauto). 
+  { left. right. vauto. }
+  right. vauto.
+Qed.  
+
+End CertT. 
